proofs/isqrt_lean4/Isqrt.lean
@@ -1,15 +1,10 @@
-import Isqrt.PythonOps
 import Isqrt.FDivLemmas
 import Isqrt.BitLengthLemmas
 import Isqrt.RecursionDepth
 import Isqrt.SizeConditions
 import Isqrt.KeyLemma
+import Isqrt.PythonOps
 import Isqrt.Algorithm
 import Isqrt.Correctness
 import Isqrt.Iterative
 import Isqrt.IterativeCorrectness
-import Isqrt.PythonOpsExcept
-import Isqrt.MonadicIsqrt
-import Isqrt.MonadicCorrectness
-import Isqrt.RecursiveExcept
-import Isqrt.RecursiveExceptCorrectness
