proofs/isqrt_lean4/IsqrtTests.lean
@@ -1,5 +1,2 @@
-import Isqrt.Tests.PythonOps
 import Isqrt.Tests.Isqrt
 import Isqrt.Tests.Iterative
-import Isqrt.Tests.MonadicIsqrt
-import Isqrt.Tests.RecursiveExcept
